@base <https://archivo.dbpedia.org/onto#> .
@prefix archivo: <> .
@prefix rdf: <http://www.w3.org/1999/02/22-rdf-syntax-ns#> .
@prefix rdfs: <http://www.w3.org/2000/01/rdf-schema#> .
@prefix owl: <http://www.w3.org/2002/07/owl#> .
@prefix xsd: <http://www.w3.org/2001/XMLSchema#> .
@prefix dc: <http://purl.org/dc/elements/1.1/> .
@prefix dct: <http://purl.org/dc/terms/> .
@prefix prov: <http://www.w3.org/ns/prov#> .
@prefix foaf: <http://xmlns.com/foaf/0.1/>.
@prefix skos: <http://www.w3.org/2004/02/skos/core#>.
@prefix vann: <http://purl.org/vocab/vann/>.


<> a owl:Ontology;
    rdfs:label "The DBpedia Archivo Ontology"@en ;
    dc:title "The DBpedia Archivo Ontology"@en ;
    dct:license <http://creativecommons.org/licenses/by/3.0/> ;		
    rdfs:comment """The Archivo Ontology lays the foundation for managing ontologies (and their metadata) on the DBpedia Databus."""@en ;
    dct:description """The Archivo Ontology lays the foundation for managing ontologies (and their metadata) on the DBpedia Databus."""@en ;
    vann:preferredNamespacePrefix "archivo";
    dct:creator <https://yum-yab.github.io/webid.ttl#this> ;
    archivo:trackThis <https://raw.githubusercontent.com/dbpedia/archivo/master/vocabulary/vocab.ttl> .


archivo:Ontology a owl:Class;
    rdfs:label "Archivo Ontology"@en;
    rdfs:comment "Everything that is considered an ontology by the DBpedia Archivo system."@en;
    dct:description "Archivo considers all instances of skos:ConceptScheme and owl:Ontology as an ontology."@en;
    rdfs:isDefinedBy <>;
    owl:unionOf (owl:Ontology skos:ConceptScheme) .


archivo:trackThis a owl:ObjectProperty;
    rdfs:label "Archivo Track This"@en;
    rdfs:comment "This property links an ontology to a file resembling the currently actively developed version of the ontology."@en;
    dct:description "This property can be used to link an ontology to the actively developed RDF file resembling the ontology, for example on github."@en;
    rdfs:isDefinedBy <> ;
    rdfs:domain archivo:Ontology;
    rdfs:range rdfs:Resource .

archivo:defines a owl:ObjectProperty;
    rdfs:label "Archivo Defines"@en;
    rdfs:comment "This property links a given resource to one that it defines."@en;
    dct:description "This property is the inverse of rdfs:isDefinedBy and can, for example, be used to link a ontology to the classes and properties it defines."@en;
    rdfs:isDefinedBy <>;
    owl:inverseOf rdfs:isDefinedBy;
    rdfs:range rdfs:Resource;
    rdfs:domain rdfs:Resource.